error boilerplate

Imp/signals.v
@@ -1,9 +1,10 @@
-From Imp Require Import header_extensible exp_ite exp_lam exp_mut.
+From Imp Require Import header_extensible exp_ite exp_lam exp_mut exp_err.
 
 Inductive exp : Type := 
     | In_exp_lam : exp_lam exp -> exp
     | In_exp_ite : exp_ite exp -> exp
     | In_exp_mut : exp_mut exp -> exp
+    | In_exp_err : exp_err exp -> exp
 .
 
 
@@ -36,12 +37,23 @@ Proof.
     - intros x y H. destruct y; (try easy).
       inversion H. easy.
 Defined.
+
+#[refine] Global Instance retract_exp_exp_err : retract (exp_err exp) exp := { 
+    retract_I := In_exp_err; 
+    retract_R := fun x => match x with In_exp_err t => Some t | _ => None end 
+    }.
+Proof.
+    - intros x. easy.
+    - intros x y H. destruct y; (try easy).
+      inversion H. easy.
+Defined.
     
 Fixpoint open_rec (k : nat) (u : exp) (e : exp) : exp := 
     match e with 
         | In_exp_lam e => open_rec_lam _ open_rec k u e
         | In_exp_ite e => open_rec_ite _ open_rec k u e
         | In_exp_mut e => open_rec_mut _ open_rec k u e
+        | In_exp_err e => open_rec_err _ open_rec k u e
     end
 .
 
@@ -51,6 +63,7 @@ Inductive lc' : nat -> exp -> Prop :=
     | lc_in_lam n e : lc'_lam _ lc' n e -> lc' n e
     | lc_in_ite n e : lc'_ite _ lc' n e -> lc' n e
     | lc_in_mut n e : lc'_mut _ lc' n e -> lc' n e
+    | lc_in_err n e : lc'_err _ lc' n e -> lc' n e
 .
 
 
@@ -58,6 +71,7 @@ Inductive value : exp -> Prop :=
     | value_in_lam (e : exp) : value_lam _ lc' e -> value e
     | value_in_ite (e : exp) : value_ite _ e -> value e
     | value_in_mut (e : exp) : value_mut _ e -> value e
+    | value_in_err (e : exp) : value_err _ e -> value e
 .
 
 
@@ -82,6 +96,13 @@ Proof.
     inversion 1; easy.
 Qed.
 
+Definition retract_lc_rev_err : forall (n : nat) (e : exp_err exp),
+        lc' n (inj e) -> lc'_err exp lc' n (inj e).
+Proof.
+    intros n e.
+    inversion 1; easy.
+Qed.
+
 Definition retract_open_rec_rev_lam : forall (n : nat) s (e : exp_lam exp),
             open_rec n s (inj e) = open_rec_lam _ open_rec n s e.
 Proof.
@@ -100,12 +121,19 @@ Proof.
     intros n s e. easy.
 Qed.
 
+Definition retract_open_rec_rev_err : forall (n : nat) s (e : exp_err exp),
+            open_rec n s (inj e) = open_rec_err _ open_rec n s e.
+Proof.
+    intros n s e. easy.
+Qed.
+
 Fixpoint lc_weaken   : forall s n m, n <= m -> lc' n s -> lc' m s.
 intros s n m n_le_m Hlc.
 inversion Hlc; subst.
 - apply (lc_weaken_lam exp _ lc_weaken lc_in_lam _) with (n := n); easy.
 - apply (lc_weaken_ite exp _ lc_weaken lc_in_ite _) with (n := n); easy.
 - apply (lc_weaken_mut exp _ lc_weaken lc_in_mut _) with (n := n); easy.
+- apply (lc_weaken_err exp _ lc_weaken lc_in_err _) with (n := n); easy.
 Qed.
 
 Fixpoint open_rec_lc : forall s t n, lc' 0 s -> lc' (S n) t -> lc' n (open_rec n s t).
@@ -115,6 +143,7 @@ inversion H2; subst.
 - apply (open_rec_lc_lam exp open_rec retract_open_rec_rev_lam lc' open_rec_lc lc_weaken lc_in_lam); easy.
 - apply (open_rec_lc_ite exp open_rec retract_open_rec_rev_ite lc' open_rec_lc lc_in_ite); easy.
 - apply (open_rec_lc_mut exp open_rec retract_open_rec_rev_mut lc' open_rec_lc lc_in_mut); easy.
+- apply (open_rec_lc_err exp open_rec retract_open_rec_rev_err lc' open_rec_lc lc_in_err); easy.
 Qed.
 
 Fixpoint value_lc : forall v, value v -> lc' 0 v.
@@ -123,6 +152,7 @@ Proof.
     - apply (value_lc_lam _ _); easy.
     - apply (value_lc_ite _ _ lc_in_ite); easy.
     - apply (value_lc_mut _ _ lc_in_mut); easy.
+    - apply (value_lc_err _ _); easy.
 Qed.
 
 From Imp Require Import context.
@@ -146,6 +176,7 @@ Inductive step : Ctx -> exp -> Ctx -> exp -> Prop :=
     | step_in_lam (c : Ctx) s c' s' : step_lam _ open_rec value _ step c s c' s' -> step c s c' s'
     | step_in_ite (c : Ctx) s c' s' : step_ite _ _                step c s c' s' -> step c s c' s'
     | step_in_mut (c : Ctx) s c' s' : step_mut _ _ _              step c s c' s' -> step c s c' s'
+    | step_in_err (c : Ctx) s c' s' : step_err _ _                step c s c' s' -> step c s c' s'
 .
 
 Definition lc := lc' 0.
@@ -162,5 +193,6 @@ Proof.
     - apply (preservation_lam exp open_rec lc' open_rec_lc lc_in_lam retract_lc_rev_lam value Ctx step preservation c s c' s'); easy.
     - apply (preservation_ite exp lc' lc_in_ite retract_lc_rev_ite Ctx step preservation c s c' s'); easy.
     - apply (preservation_mut exp lc' lc_in_mut retract_lc_rev_mut value value_lc Ctx step preservation c s c' s'); easy.
+    - apply (preservation_err exp lc' lc_in_err retract_lc_rev_err Ctx step preservation c s c' s'); easy.
 Defined.
 
