Imp/features/exp_err.v
@@ -1,0 +1,82 @@
+From Imp Require Export header_extensible.
+
+Section exp_err.
+    Variable exp : Type.
+
+    Inductive exp_err : Type := 
+        | err (e : exp) : exp_err
+    .
+
+    Context `{retract exp_err exp}.
+
+    Definition err_  (e : exp) : _ := inj (err e).
+
+    Variable open_rec : nat -> exp -> exp -> exp.
+
+    Definition open_rec_err (k : nat) (s : exp) (t : exp_err) : exp := 
+        match t with 
+            | err e => err_ (open_rec k s e)
+        end.
+    
+    Variable retract_open_rec : forall (n : nat) s (e : exp_err),
+          open_rec n s (inj e) = open_rec_err n s e.
+
+    Variable lc' : nat -> exp -> Prop.
+    Variable open_rec_lc :forall s t n, lc' 0 s -> lc' (S n) t -> lc' n (open_rec n s t).
+    Variable lc_weaken   : forall s n m, n <= m  -> lc' n s -> lc' m s.
+    
+    Inductive lc'_err : nat -> exp -> Prop := 
+        | lc_err n e : lc' n e -> lc'_err n (err_ e)
+    .
+
+    Variable retract_lc: forall n e, lc'_err n e -> lc' n e.
+    Variable retract_lc_rev: forall n e, lc' n (inj e) -> lc'_err n (inj e).
+
+    Definition lc_weaken_err : forall s n m, n <= m -> lc'_err n s -> lc' m s.
+    Proof.
+        intros s n m n_le_m.
+        induction 1. apply retract_lc. constructor. 
+        apply lc_weaken with (n := n); easy.
+    Defined.
+
+    Definition open_rec_lc_err : forall s t n, lc' 0 s -> lc'_err (S n) t -> lc' n (open_rec n s t).
+    Proof.
+        intros s t n lc_s lc_err.
+        inversion lc_err. subst. unfold err_. rewrite retract_open_rec.
+        simpl. apply retract_lc. constructor.
+        apply open_rec_lc; try easy.
+    Defined.
+    
+    Variable value : exp -> Prop.
+    Variable value_lc : forall v, value v -> lc' 0 v.
+
+    Inductive value_err : exp -> Prop := 
+    .
+
+    Definition value_lc_err : forall v, value_err v -> lc' 0 v.
+    Proof.
+        intros v. induction 1.
+    Defined.
+
+    Variable Ctx : Type.
+    Variable step : Ctx -> exp -> Ctx -> exp -> Prop.
+    Variable preservation : forall c e c' e', lc' 0 e -> step c e c' e' -> lc' 0 e'.
+    
+
+    Inductive step_err : Ctx -> exp -> Ctx -> exp -> Prop :=
+        | step_err_red c e c' e' : step c e c' e' -> step_err c (err_ e) c' (err_ e')
+    .
+
+    
+    Definition preservation_err : forall c e c' e', lc' 0 e -> step_err c e c' e' -> lc' 0 e'.
+    Proof. 
+        intros c e c' e' lc_e.
+        induction 1.
+        apply retract_lc_rev in lc_e.
+        inversion lc_e. subst.
+        apply retract_inj in H1. inversion H1. subst.
+        apply retract_lc. constructor.
+        apply (preservation c e c' e'); easy.
+    Defined.
+        
+End exp_err.
